examples/ChildParentNames.v
@@ -1,0 +1,8 @@
+Require Import String.
+
+Local Open Scope string.
+Definition rqFromCToPRule := "rqFromCToP".
+Definition rsFromCToPRule := "rsFromCToP".
+Definition fromPToCRule := "fromPToC".
+Close Scope string.
+
