examples/FifoNames.v
@@ -1,0 +1,13 @@
+Require Import String.
+
+Local Open Scope string.
+Definition elt := "elt".
+Definition enqName := "enq".
+Definition deqName := "deq".
+Definition enqP := "enqP".
+Definition deqP := "deqP".
+Definition empty := "empty".
+Definition full := "full".
+Definition firstEltName := "firstElt".
+Close Scope string.
+
