examples/L1Cache.v
@@ -2,7 +2,7 @@ Require Import Ascii Bool String List.
 Require Import Lib.CommonTactics Lib.ilist Lib.Word Lib.Indexer Lib.StringBound.
 Require Import Kami.Syntax Kami.Notations Kami.Semantics.
 Require Import Kami.ParametricEquiv Kami.Wf Kami.ParametricWf Kami.Tactics.
-Require Import Ex.Msi Ex.MemTypes Ex.RegFile Kami.ParametricSyntax.
+Require Import Ex.Msi Ex.MemTypes Ex.RegFile Kami.ParametricSyntax Ex.FifoNames Ex.Names Ex.L1CacheNames.
 
 Set Implicit Arguments.
 
@@ -27,21 +27,23 @@ Section L1Cache.
   Definition RqToP := Ex.MemTypes.RqToP TagIdx Id.
   Definition RsToP := Ex.MemTypes.RsToP LgDataBytes LgNumDatas TagIdx.
 
-  Definition rqFromProcPop := MethodSig "rqFromProc"--"deq" (Void): RqFromProc.
-  Definition rqFromProcFirst := MethodSig "rqFromProc"--"firstElt" (Void): RqFromProc.
-  Definition fromPPop := MethodSig "fromParent"--"deq" (Void): FromP.
+  Definition rqFromProcPop := MethodSig (rqFromProc -- deqName) (Void): RqFromProc.
+  Definition rqFromProcFirst := MethodSig (rqFromProc -- firstEltName) (Void): RqFromProc.
+  Definition fromPPop := MethodSig (fromParent -- deqName) (Void): FromP.
 
-  Definition rsToProcEnq := MethodSig "rsToProc"--"enq" (RsToProc): Void.
-  Definition rqToPEnq := MethodSig "rqToParent"--"enq" (RqToP): Void.
-  Definition rsToPEnq := MethodSig "rsToParent"--"enq" (RsToP): Void.
+  Definition rsToProcEnq := MethodSig (rsToProc -- enqName) (RsToProc): Void.
+  Definition rqToPEnq := MethodSig (rqToParent -- enqName) (RqToP): Void.
+  Definition rsToPEnq := MethodSig (rsToParent -- enqName) (RsToP): Void.
 
-  Definition readLine := MethodSig "line"--"read" (Idx): Line.
-  Definition writeLine := MethodSig "line"--"write" (WritePort IdxBits Line): Void.
-  Definition readTag := MethodSig "tag"--"read" (Idx): Tag.
-  Definition writeTag := MethodSig "tag"--"write" (WritePort IdxBits Tag): Void.
-  Definition readCs := MethodSig "cs"--"read" (Idx): Msi.
-  Definition writeCs := MethodSig "cs"--"write" (WritePort IdxBits Msi): Void.
+  Definition lineRead := MethodSig (line -- read) (Idx): Line.
+  Definition lineWrite := MethodSig (line -- write) (WritePort IdxBits Line): Void.
+  Definition tagRead := MethodSig (tag -- read) (Idx): Tag.
+  Definition tagWrite := MethodSig (tag -- write) (WritePort IdxBits Tag): Void.
+  Definition csRead := MethodSig (cs -- read) (Idx): Msi.
+  Definition csWrite := MethodSig (cs --write) (WritePort IdxBits Msi): Void.
 
+
+  
   Section UtilFunctions.
     Variable var: Kind -> Type.
     Definition getTagIdx (x: (Addr @ var)%kami): (TagIdx @ var)%kami :=
@@ -69,208 +71,171 @@ Section L1Cache.
 
   Definition l1Cache :=
     SIN {
-        Register "procRqValid": Bool <- false
-        with Register "procRqReplace": Bool <- false
-        with Register "procRqWait": Bool <- false
-        with Register "procRq": RqFromProc <- Default
+        Register procRqValidReg: Bool <- false
+        with Register procRqReplaceReg: Bool <- false
+        with Register procRqWaitReg: Bool <- false
+        with Register procRqReg: RqFromProc <- Default
 
-        (*                                 
-        with Rule "ldHit" :=
-          Read valid <- "procRqValid";
-          Assert !#valid;
-          Call rq <- rqFromProcPop();
-          Assert !#rq@."op";
-          LET idx <- getIdx #rq@."addr";
-          Call tag <- readTag(#idx);
-          Call cs <- readCs(#idx);
-          Assert ((#cs >= $ Sh) && #tag == getTag #rq@."addr");
-          Call line <- readLine(#idx);
-          Call rsToProcEnq(STRUCT {
-                               "data" ::= #line@[getOffset #rq@."addr"]
-                               (* "id" ::= #rq@."id" *)
-                          });
-          Retv
-
-        with Rule "stHit" :=
-          Read valid <- "procRqValid";
-          Assert !#valid;
-          Call rq <- rqFromProcPop();
-          Assert #rq@."op";
-          LET idx <- getIdx #rq@."addr";
-          Call tag <- readTag(#idx);
-          Call cs <- readCs(#idx);
-          Assert (#cs == $ Mod && #tag == getTag #rq@."addr");
-          Call line <- readLine(#idx);
-          LET offset <- getOffset #rq@."addr";
-          Call rsToProcEnq(STRUCT {
-                               "data" ::= $$Default
-                               (* "id" ::= #rq@."id" *)
-                          });
-          LET updLine <- #line@[#offset <- #rq@."data"];
-          Call writeLine(STRUCT{"addr" ::= #idx; "data" ::= #updLine});
-          Retv
-        *)
-
-        with Rule "l1MissByState" :=
-          Read valid <- "procRqValid";
+        with Rule l1MissByState :=
+          Read valid <- procRqValidReg;
           Assert !#valid;
           Call rq <- rqFromProcFirst();
-          LET idx <- getIdx #rq@."addr";
-          Call tag <- readTag(#idx);
-          Call cs <- readCs(#idx);
-          Assert (#tag == getTag #rq@."addr" && #cs == $ Sh && #rq@."op");
-          Write "procRqValid" <- $$ true;
-          Write "procRqReplace" <- $$ false;
-          Write "procRqWait" <- $$ false;
-          Write "procRq" <- #rq;
+          LET idx <- getIdx #rq@.addr;
+          Call tag <- tagRead(#idx);
+          Call cs <- csRead(#idx);
+          Assert (#tag == getTag #rq@.addr && #cs == $ Sh && #rq@.op);
+          Write procRqValidReg <- $$ true;
+          Write procRqReplaceReg <- $$ false;
+          Write procRqWaitReg <- $$ false;
+          Write procRqReg <- #rq;
           Retv
 
-        with Rule "l1MissByLine" :=
-          Read valid <- "procRqValid";
+        with Rule l1MissByLine :=
+          Read valid <- procRqValidReg;
           Assert !#valid;
           Call rq <- rqFromProcFirst();
-          LET idx <- getIdx #rq@."addr";
-          Call tag <- readTag(#idx);
-          Call cs <- readCs(#idx);
-          Assert (!(#tag == getTag #rq@."addr") || #cs == $ Inv);
-          Write "procRqValid" <- $$ true;
-          Write "procRqReplace" <- $$ true;
-          Write "procRqWait" <- $$ false;
-          Write "procRq" <- #rq;
+          LET idx <- getIdx #rq@.addr;
+          Call tag <- tagRead(#idx);
+          Call cs <- csRead(#idx);
+          Assert (!(#tag == getTag #rq@.addr) || #cs == $ Inv);
+          Write procRqValidReg <- $$ true;
+          Write procRqReplaceReg <- $$ true;
+          Write procRqWaitReg <- $$ false;
+          Write procRqReg <- #rq;
           Retv
 
-        with Rule "l1Hit" :=
-          Read valid <- "procRqValid";
+        with Rule l1Hit :=
+          Read valid <- procRqValidReg;
           Assert !#valid;
           Call rq <- rqFromProcFirst();
-          LET idx <- getIdx #rq@."addr";
-          Call tag <- readTag(#idx);
-          Call cs <- readCs(#idx);
-          Assert ((#tag == getTag #rq@."addr") &&
-                  (#cs == $ Sh && !#rq@."op" || #cs == $ Mod && #rq@."op"));
-          Write "procRqValid" <- $$ true;
-          Write "procRqReplace" <- $$ false;
-          Write "procRqWait" <- $$ false;
-          Write "procRq" <- #rq;
+          LET idx <- getIdx #rq@.addr;
+          Call tag <- tagRead(#idx);
+          Call cs <- csRead(#idx);
+          Assert ((#tag == getTag #rq@.addr) &&
+                  (#cs == $ Sh && !#rq@.op || #cs == $ Mod && #rq@.op));
+          Write procRqValidReg <- $$ true;
+          Write procRqReplaceReg <- $$ false;
+          Write procRqWaitReg <- $$ false;
+          Write procRqReg <- #rq;
           Retv
 
 
-        with Rule "writeback" :=
-          Read valid <- "procRqValid";
+        with Rule writeback :=
+          Read valid <- procRqValidReg;
           Assert #valid;
-          Read replace <- "procRqReplace";
+          Read replace <- procRqReplaceReg;
           Assert #replace;
-          Read rq: RqFromProc <- "procRq";
-          LET idx <- getIdx #rq@."addr";
-          Call tag <- readTag(#idx);
-          Call cs <- readCs(#idx);
-          Call line <- readLine(#idx);
+          Read rq: RqFromProc <- procRqReg;
+          LET idx <- getIdx #rq@.addr;
+          Call tag <- tagRead(#idx);
+          Call cs <- csRead(#idx);
+          Call lineT <- lineRead(#idx);
           If !(#cs == $ Inv)
-          then (Call rsToPEnq(STRUCT{"addr" ::= makeTagIdx #tag #idx; "to" ::= $ Inv; "line" ::= #line; "isVol" ::= $$ true}); Retv)
+          then (Call rsToPEnq(STRUCT{addr ::= makeTagIdx #tag #idx; to ::= $ Inv; line ::= #lineT; isVol ::= $$ true}); Retv)
           else Retv as _;
-          Call writeCs(STRUCT{ "addr" ::= #idx; "data" ::= $ Inv});
-          Write "procRqReplace" <- $$ false;
+          Call csWrite(STRUCT{ addr ::= #idx; data ::= $ Inv});
+          Write procRqReplaceReg <- $$ false;
           Retv
 
-        with Rule "upgRq" :=
-          Read valid <- "procRqValid";
+        with Rule upgRq :=
+          Read valid <- procRqValidReg;
           Assert #valid;
-          Read replace <- "procRqReplace";
+          Read replace <- procRqReplaceReg;
           Assert !#replace;
-          Read rq: RqFromProc <- "procRq";
-          LET idx <- getIdx #rq@."addr";
-          Call cs <- readCs(#idx);
-          LET toS: Msi <- IF #rq@."op" then $ Mod else $ Sh;
-          Read wait <- "procRqWait";
-          Call tag <- readTag(#idx);
+          Read rq: RqFromProc <- procRqReg;
+          LET idx <- getIdx #rq@.addr;
+          Call cs <- csRead(#idx);
+          LET toS: Msi <- IF #rq@.op then $ Mod else $ Sh;
+          Read wait <- procRqWaitReg;
+          Call tag <- tagRead(#idx);
           Assert (!#wait && (#cs == $ Msi.Inv ||
-                                      ((#tag == getTag #rq@."addr") && (#cs < #toS))));
-          Call rqToPEnq(STRUCT{"addr" ::= getTagIdx #rq@."addr"; "from" ::= #cs; "to" ::= #toS; "id" ::= $$ Default});
-          Write "procRqWait" <- $$ true;
+                                      ((#tag == getTag #rq@.addr) && (#cs < #toS))));
+          Call rqToPEnq(STRUCT{addr ::= getTagIdx #rq@.addr; from ::= #cs; to ::= #toS; id ::= $$ Default});
+          Write procRqWaitReg <- $$ true;
           Retv
 
-        with Rule "upgRs" :=
+        with Rule upgRs :=
           Call fromP <- fromPPop();
-          Assert !#fromP@."isRq";
-          LET idx <- getIdxFromTagIdx #fromP@."addr";
-          Call cs <- readCs(#idx);
-          Call writeCs(STRUCT{"addr" ::= #idx; "data" ::= #fromP@."to"});
-          Call writeTag(STRUCT{"addr" ::= #idx; "data" ::= getTagFromTagIdx #fromP@."addr"});
-          Write "procRqWait" <- $$ false;
-          If #cs == $ Inv then Call writeLine(STRUCT{"addr" ::= #idx; "data" ::= #fromP@."line"}); Retv
+          Assert !#fromP@.isRq;
+          LET idx <- getIdxFromTagIdx #fromP@.addr;
+          Call cs <- csRead(#idx);
+          Call csWrite(STRUCT{addr ::= #idx; data ::= #fromP@.to});
+          Call tagWrite(STRUCT{addr ::= #idx; data ::= getTagFromTagIdx #fromP@.addr});
+          Write procRqWaitReg <- $$ false;
+          If #cs == $ Inv then Call lineWrite(STRUCT{addr ::= #idx; data ::= #fromP@.line}); Retv
                           else Retv as _;
           Retv
 
-        with Rule "ld" :=
-          Read valid <- "procRqValid";
+        with Rule ld :=
+          Read valid <- procRqValidReg;
           Assert #valid;
-          Read replace <- "procRqReplace";
+          Read replace <- procRqReplaceReg;
           Assert !#replace;
-          Read rq: RqFromProc <- "procRq";
-          Assert !#rq@."op";
-          LET idx <- getIdx #rq@."addr";
-          Call tag <- readTag(#idx);
-          Assert #tag == getTag (#rq@."addr");
-          Call cs <- readCs(#idx);
+          Read rq: RqFromProc <- procRqReg;
+          Assert !#rq@.op;
+          LET idx <- getIdx #rq@.addr;
+          Call tag <- tagRead(#idx);
+          Assert #tag == getTag (#rq@.addr);
+          Call cs <- csRead(#idx);
           Assert #cs >= $ Sh;
-          Call line <- readLine(#idx);
-          Write "procRqValid" <- $$ false;
+          Call line <- lineRead(#idx);
+          Write procRqValidReg <- $$ false;
           Call rsToProcEnq(STRUCT {
-                               "data" ::= #line@[getOffset #rq@."addr"]
-                               (* "id" ::= #rq@."id" *)
+                               data ::= #line@[getOffset #rq@.addr]
+                               (* id ::= #rq@.id *)
                           });
           Call rq' <- rqFromProcPop();
           Assert #rq == #rq';
           Retv
 
-        with Rule "st" :=
-          Read valid <- "procRqValid";
+        with Rule st :=
+          Read valid <- procRqValidReg;
           Assert #valid;
-          Read replace <- "procRqReplace";
+          Read replace <- procRqReplaceReg;
           Assert !#replace;
-          Read rq: RqFromProc <- "procRq";
-          Assert #rq@."op";
-          LET idx <- getIdx #rq@."addr";
-          Call tag <- readTag(#idx);
-          Assert #tag == getTag (#rq@."addr");
-          Call cs <- readCs(#idx);
+          Read rq: RqFromProc <- procRqReg;
+          Assert #rq@.op;
+          LET idx <- getIdx #rq@.addr;
+          Call tag <- tagRead(#idx);
+          Assert #tag == getTag (#rq@.addr);
+          Call cs <- csRead(#idx);
           Assert #cs == $ Mod;
-          Call line <- readLine(#idx);
-          Write "procRqValid" <- $$ false;
-          LET offset <- getOffset #rq@."addr";
+          Call line <- lineRead(#idx);
+          Write procRqValidReg <- $$ false;
+          LET offset <- getOffset #rq@.addr;
           Call rsToProcEnq(STRUCT {
-                               "data" ::= $$Default
-                               (* "id" ::= #rq@."id" *)
+                               data ::= $$Default
+                               (* id ::= #rq@.id *)
                           });
-          Call writeLine(STRUCT{"addr" ::= #idx; "data" ::= #line@[#offset <- #rq@."data"]});
+          Call lineWrite(STRUCT{addr ::= #idx; data ::= #line@[#offset <- #rq@.data]});
           Call rq' <- rqFromProcPop();
           Assert #rq == #rq';
           Retv
 
-        with Rule "drop" :=
+        with Rule drop :=
           Call fromP <- fromPPop();
-          Assert #fromP@."isRq";
-          LET idx <- getIdxFromTagIdx #fromP@."addr";
-          Call cs <- readCs(#idx);
-          Call tag <- readTag(#idx);
-          Assert (#cs <= #fromP@."to") || !(#tag == getTagFromTagIdx #fromP@."addr");
+          Assert #fromP@.isRq;
+          LET idx <- getIdxFromTagIdx #fromP@.addr;
+          Call cs <- csRead(#idx);
+          Call tag <- tagRead(#idx);
+          Assert (#cs <= #fromP@.to) || !(#tag == getTagFromTagIdx #fromP@.addr);
           Retv
 
-        with Rule "pProcess" :=
+        with Rule pProcess :=
           Call fromP <- fromPPop();
-          Assert #fromP@."isRq";
-          LET idx <- getIdxFromTagIdx #fromP@."addr";
-          Call cs <- readCs(#idx);
-          Call tag <- readTag(#idx);
-          Call line <- readLine(#idx);
-          Assert (#cs > #fromP@."to") && (#tag == getTagFromTagIdx #fromP@."addr");
-          Read valid <- "procRqValid";
-          Read wait <- "procRqWait";
-          Read procRq: RqFromProc <- "procRq";
-          Assert !(#valid && !#wait && getTagIdx #procRq@."addr" == #fromP@."addr" &&
-                  (#procRq@."op" && #cs == $ Mod || (!#procRq@."op" && #cs == $ Sh)));
-          Call rsToPEnq(STRUCT{"addr" ::= #fromP@."addr"; "to" ::= #fromP@."to"; "line" ::= #line; "isVol" ::= $$ false});
-          Call writeCs(STRUCT{"addr" ::= #idx; "data" ::= #fromP@."to"});
+          Assert #fromP@.isRq;
+          LET idx <- getIdxFromTagIdx #fromP@.addr;
+          Call cs <- csRead(#idx);
+          Call tag <- tagRead(#idx);
+          Call lineT <- lineRead(#idx);
+          Assert (#cs > #fromP@.to) && (#tag == getTagFromTagIdx #fromP@.addr);
+          Read valid <- procRqValidReg;
+          Read wait <- procRqWaitReg;
+          Read procRq: RqFromProc <- procRqReg;
+          Assert !(#valid && !#wait && getTagIdx #procRq@.addr == #fromP@.addr &&
+                  (#procRq@.op && #cs == $ Mod || (!#procRq@.op && #cs == $ Sh)));
+          Call rsToPEnq(STRUCT{addr ::= #fromP@.addr; to ::= #fromP@.to; line ::= #lineT; isVol ::= $$ false});
+          Call csWrite(STRUCT{addr ::= #idx; data ::= #fromP@.to});
           Retv
       }.
 End L1Cache.
@@ -278,7 +243,7 @@ End L1Cache.
 Hint Unfold AddrBits Addr Tag Idx TagIdx Data Offset Line : MethDefs.
 Hint Unfold RqFromProc RsToProc FromP RqFromP RsFromP RqToP RsToP : MethDefs.
 Hint Unfold rqFromProcPop fromPPop rsToProcEnq rqToPEnq rsToPEnq : MethDefs.
-Hint Unfold readLine writeLine readTag writeTag readCs writeCs : MethDefs.
+Hint Unfold lineRead lineWrite tagRead tagWrite csRead csWrite : MethDefs.
 Hint Unfold getTagIdx getTag getIdx getOffset makeTagIdx : MethDefs.
 
 Hint Unfold l1Cache : ModuleDefs.
