examples/MemDir.v
@@ -2,7 +2,7 @@ Require Import Ascii Bool String List.
 Require Import Lib.CommonTactics Lib.ilist Lib.Word Lib.Indexer Lib.StringBound.
 Require Import Kami.Syntax Kami.Notations Kami.Semantics Kami.ParametricEquiv.
 Require Import Kami.Wf Kami.ParametricWf Kami.Tactics.
-Require Import Ex.Msi Ex.MemTypes Ex.RegFile.
+Require Import Ex.Msi Ex.MemTypes Ex.RegFile Ex.Names Ex.FifoNames Ex.MemDirNames.
 
 Set Implicit Arguments.
 
@@ -39,21 +39,21 @@ Section Mem.
   Definition RsFromC := Ex.MemTypes.RsFromC LgDataBytes LgNumDatas LgNumChildren Addr.
   Definition FromP := Ex.MemTypes.FromP LgDataBytes LgNumDatas Addr Id.
   Definition ToC := Ex.MemTypes.ToC LgDataBytes LgNumDatas LgNumChildren Addr Id.
+  
+  Definition rqFromCPop := MethodSig (rqFromChild -- deqName) (Void): RqFromC.
+  Definition rqFromCFirst := MethodSig (rqFromChild -- firstEltName) (Void): RqFromC.
+  Definition rsFromCPop := MethodSig (rsFromChild -- deqName) (Void): RsFromC.
 
-  Definition rqFromCPop := MethodSig "rqFromChild"--"deq" (Void): RqFromC.
-  Definition rqFromCFirst := MethodSig "rqFromChild"--"firstElt" (Void): RqFromC.
-  Definition rsFromCPop := MethodSig "rsFromChild"--"deq" (Void): RsFromC.
-
-  Definition toCEnq := MethodSig "toChild"--"enq" (ToC): Void.
+  Definition toCEnq := MethodSig (toChild -- enqName) (ToC): Void.
 
   Definition Dir := Vector Msi LgNumChildren.
   
   Definition Dirw := Vector Bool LgNumChildren.
   
-  Definition readLine := MethodSig "mline"--"read" (Idx): Line.
-  Definition writeLine := MethodSig "mline"--"write" (WritePort IdxBits Line): Void.
-  Definition readDir := MethodSig "mcs"--"read" (Idx): Dir.
-  Definition writeDir := MethodSig "mcs"--"write" (WritePort IdxBits Dir): Void.
+  Definition lineRead := MethodSig (mline -- read) (Idx): Line.
+  Definition lineWrite := MethodSig (mline -- write) (WritePort IdxBits Line): Void.
+  Definition dirRead := MethodSig (mcs -- read) (Idx): Dir.
+  Definition dirWrite := MethodSig (mcs -- write) (WritePort IdxBits Dir): Void.
 
   Definition Child := MemTypes.Child LgNumChildren.
   
@@ -77,10 +77,10 @@ Section Mem.
     Definition findIncompat (c: (Child@var)%kami) (x: (Msi@var)%kami)
                (dir: (Dir@var)%kami) (dirw: (Dirw@var)%kami): ((Maybe Child)@var)%kami :=
       foldInc (fun idx (old: ((Maybe Child) @ var)%kami) =>
-                 IF !old@."valid" && !(c == idx) && !(isCompat x (dir@[idx])%kami) && !(dirw@[idx])%kami
-                 then STRUCT{"valid" ::= $$ true ; "value" ::= idx}
+                 IF !old@.isValid && !(c == idx) && !(isCompat x (dir@[idx])%kami) && !(dirw@[idx])%kami
+                 then STRUCT{isValid ::= $$ true ; value ::= idx}
                else old)%kami_expr
-              (STRUCT{"valid" ::= $$ false; "value" ::= $$ Default})%kami_expr.
+              (STRUCT{isValid ::= $$ false; value ::= $$ Default})%kami_expr.
     
   End UtilFunctions.
 
@@ -88,94 +88,94 @@ Section Mem.
 
   Definition memDir :=
     META {
-        Register "cRqValid": Bool <- false
-        with Register "cRqDirw": Dirw <- dirwInit
-        with Register "cRq": RqFromC <- Default
+        Register cRqValidReg: Bool <- false
+        with Register cRqDirwReg: Dirw <- dirwInit
+        with Register cRqReg: RqFromC <- Default
 
-        with Rule "missByState" :=
-          Read valid <- "cRqValid";
+        with Rule missByState :=
+          Read valid <- cRqValidReg;
           Assert !#valid;
           Call rqChild <- rqFromCFirst();
-          LET c <- #rqChild@."child";
-          LET rq: RqToP <- #rqChild@."rq";
-          LET idx <- getIdx (#rq@."addr");
-          Call dir <- readDir(#idx);
-          Assert (#dir@[#c] <= #rq@."from");
-          Write "cRqValid" <- $$ true;
+          LET c <- #rqChild@.child;
+          LET rqT: RqToP <- #rqChild@.rq;
+          LET idx <- getIdx (#rqT@.addr);
+          Call dir <- dirRead(#idx);
+          Assert (#dir@[#c] <= #rqT@.from);
+          Write cRqValidReg <- $$ true;
           LET dirw: Dirw <- VEC (replicate ($$ false) _);
-          Write "cRqDirw" <- #dirw;
-          Write "cRq" <- #rqChild;
+          Write cRqDirwReg <- #dirw;
+          Write cRqReg <- #rqChild;
           Retv
 
-        with Rule "dwnRq" :=
-          Read valid <- "cRqValid";
+        with Rule dwnRq :=
+          Read valid <- cRqValidReg;
           Assert #valid;
           Call rqChild <- rqFromCFirst();
-          LET c <- #rqChild@."child";
-          LET rq: RqToP <- #rqChild@."rq";
-          Call dir <- readDir(getIdx #rq@."addr");
-          Read dirw <- "cRqDirw";
-          LET i <- findIncompat #c #rq@."to" #dir #dirw;
-          Assert #i@."valid";
-          LET rq': FromP <- STRUCT{"isRq" ::= $$ true; "addr" ::= #rq@."addr"; "to" ::= toCompat #rq@."to"; "line" ::= $$ Default; "id" ::= $$ Default};
-          Call toCEnq(STRUCT{"child" ::= #c; "msg" ::= #rq'});
+          LET c <- #rqChild@.child;
+          LET rqT: RqToP <- #rqChild@.rq;
+          Call dir <- dirRead(getIdx #rqT@.addr);
+          Read dirw <- cRqDirwReg;
+          LET i <- findIncompat #c #rqT@.to #dir #dirw;
+          Assert #i@.isValid;
+          LET rq': FromP <- STRUCT{isRq ::= $$ true; addr ::= #rqT@.addr; to ::= toCompat #rqT@.to; line ::= $$ Default; id ::= $$ Default};
+          Call toCEnq(STRUCT{child ::= #c; msg ::= #rq'});
           LET dirw' <- #dirw@[#c <- $$ true];
-          Write "cRqDirw" <- #dirw';
+          Write cRqDirwReg <- #dirw';
           Retv
 
-        with Rule "dwnRs_wait" :=
+        with Rule dwnRs_wait :=
           Call rsChild <- rsFromCPop();
-          LET c <- #rsChild@."child";
-          LET rs: RsToP <- #rsChild@."rs";
-          LET idx <- getIdx #rs@."addr";
-          Call dir <- readDir(#idx);
-          LET dir' <- #dir@[#c <- #rs@."to"];
-          Call writeDir(STRUCT{"addr" ::= #idx; "data" ::= #dir'});
+          LET c <- #rsChild@.child;
+          LET rs: RsToP <- #rsChild@.rs;
+          LET idx <- getIdx #rs@.addr;
+          Call dir <- dirRead(#idx);
+          LET dir' <- #dir@[#c <- #rs@.to];
+          Call dirWrite(STRUCT{addr ::= #idx; data ::= #dir'});
           If #dir@[#c] == $ Mod
-          then Call writeLine(STRUCT{"addr" ::= #idx; "data" ::= #rs@."line"}); Retv
+          then Call lineWrite(STRUCT{addr ::= #idx; data ::= #rs@.line}); Retv
           else Retv as _;
-          Read rqChild: RqFromC <- "cRq";
-          LET rq: RqToP <- #rqChild@."rq";
-          Read valid <- "cRqValid";
-          Assert #valid && #rq@."addr" == #rs@."addr";
-          Read dirw <- "cRqDirw";
+          Read rqChild: RqFromC <- cRqReg;
+          LET rq: RqToP <- #rqChild@.rq;
+          Read valid <- cRqValidReg;
+          Assert #valid && #rq@.addr == #rs@.addr;
+          Read dirw <- cRqDirwReg;
           LET dirw' <- #dirw@[#c <- $$ false];
-          Write "cRqDirw" <- #dirw';
+          Write cRqDirwReg <- #dirw';
           Retv
 
-        with Rule "dwnRs_noWait" :=
+        with Rule dwnRs_noWait :=
           Call rsChild <- rsFromCPop();
-          LET c <- #rsChild@."child";
-          LET rs: RsToP <- #rsChild@."rs";
-          LET idx <- getIdx #rs@."addr";
-          Call dir <- readDir(#idx);
-          LET dir' <- #dir@[#c <- #rs@."to"];
-          Call writeDir(STRUCT{"addr" ::= #idx; "data" ::= #dir'});
+          LET c <- #rsChild@.child;
+          LET rs: RsToP <- #rsChild@.rs;
+          LET idx <- getIdx #rs@.addr;
+          Call dir <- dirRead(#idx);
+          LET dir' <- #dir@[#c <- #rs@.to];
+          Call dirWrite(STRUCT{addr ::= #idx; data ::= #dir'});
           If #dir@[#c] == $ Mod
-          then Call writeLine(STRUCT{"addr" ::= #idx; "data" ::= #rs@."line"}); Retv
+          then Call lineWrite(STRUCT{addr ::= #idx; data ::= #rs@.line}); Retv
           else Retv as _;
-          Read rqChild: RqFromC <- "cRq";
-          LET rq: RqToP <- #rqChild@."rq";
-          Read valid <- "cRqValid";
-          Assert !(#valid && #rq@."addr" == #rs@."addr");
+          Read rqChild: RqFromC <- cRqReg;
+          LET rq: RqToP <- #rqChild@.rq;
+          Read valid <- cRqValidReg;
+          Assert !(#valid && #rq@.addr == #rs@.addr);
           Retv
             
-        with Rule "deferred" :=
-          Read valid <- "cRqValid";
+        with Rule deferred :=
+          Read valid <- cRqValidReg;
           Assert #valid;
           Call rqChild <- rqFromCPop();
-          LET c <- #rqChild@."child";
-          LET rq: RqToP <- #rqChild@."rq";
-          LET idx <- getIdx (#rq@."addr");
-          Call dir <- readDir(#idx);
-          Assert #dir@[#c] <= #rq@."from";
-          Assert (othersCompat #c #rq@."to" #dir);
-          Call line <- readLine(#idx);
-          LET rs: FromP <- STRUCT{"isRq" ::= $$ false; "addr" ::= #rq@."addr"; "to" ::= #rq@."to"; "line" ::= #line; "id" ::= #rq@."id"};
-          Call toCEnq(STRUCT{"child" ::= #c; "msg" ::= #rs});
-          LET dir' <- #dir@[#c <- #rq@."to"];
-          Call writeDir(STRUCT{"addr" ::= #idx; "data" ::= #dir'});
-          Write "cRqValid" <- $$ false;
+          LET c <- #rqChild@.child;
+          LET rq: RqToP <- #rqChild@.rq;
+          LET idx <- getIdx (#rq@.addr);
+          Call dir <- dirRead(#idx);
+          Assert #dir@[#c] <= #rq@.from;
+          Assert (othersCompat #c #rq@.to #dir);
+          Call lineT <- lineRead(#idx);
+          LET rs: FromP <- STRUCT{isRq ::= $$ false; addr ::= #rq@.addr; to ::= #rq@.to; line ::= #lineT; id ::= #rq@.id};
+          Call toCEnq(STRUCT{child ::= #c; msg ::= #rs});
+          LET dir' <- #dir@[#c <- #rq@.to];
+          Call dirWrite(STRUCT{addr ::= #idx; data ::= #dir'});
+          Write cRqValidReg <- $$ false;
           Retv
       }.
 End Mem.
@@ -183,7 +183,7 @@ End Mem.
 Hint Unfold AddrBits Addr Idx Data Offset Line : MethDefs.
 Hint Unfold RqToP RqFromC RsToP RsFromC FromP ToC : MethDefs.
 Hint Unfold rqFromCPop rsFromCPop toCEnq Dir Dirw : MethDefs.
-Hint Unfold readLine writeLine readDir writeDir Child : MethDefs.
+Hint Unfold lineRead lineWrite dirRead dirWrite Child : MethDefs.
 Hint Unfold getIdx getOffset getAddr othersCompat findIncompat dirwInit : MethDefs.
 
 Hint Unfold memDir : ModuleDefs.
