examples/MemDirNames.v
@@ -1,0 +1,13 @@
+Require Import String.
+
+Local Open Scope string.
+Definition cRqValidReg := "cRqValid".
+Definition cRqDirwReg := "cRqDirw".
+Definition cRqReg := "cRqReg".
+Definition missByState := "missByState".
+Definition dwnRq := "dwnRq".
+Definition dwnRs_wait := "dwnRs_wait".
+Definition dwnRs_noWait := "dwnRs_noWait".
+Definition deferred := "deferred".
+Close Scope string.
+
