examples/Names.v
@@ -1,0 +1,17 @@
+Require Import String.
+
+Local Open Scope string.
+Definition rqFromProc := "rqFromProc".
+Definition rsToProc := "rsToProc".
+Definition rqToParent := "rqToParent".
+Definition rsToParent := "rsToParent".
+Definition rqFromChild := "rqFromChild".
+Definition rsFromChild := "rsFromChild".
+Definition fromParent := "fromParent".
+Definition toChild := "toChild".
+Definition line := "line".
+Definition tag := "tag".
+Definition cs := "cs".
+Definition mcs := "mcs".
+Definition mline := "mline".
+Close Scope string.
